{\bf 07.05} \quad

$ \frac{\sum_{i=1}^{n} (Z_i+ \frac{1}{n} ) }{\sqrt{n}} =\frac{ (\sum_{i=1}^{n} Z_i)  + \frac{1}{n} \times n }{n}=\frac{\sum_{i=1}^{n} Z_i}{\sqrt{n}} + \frac{1}{\sqrt{n}} $ 
\par

$ M_{\frac{\sum_{i=1}^{n} (Z_i+ \frac{1}{n} ) }{\sqrt{n}} } (t)= M_{\frac{\sum_{i=1}^{n} Z_i}{\sqrt{n}} + \frac{1}{\sqrt{n}} } (t) = E[e^  { \frac{1}{\sqrt{n}} \times t} ] \times (M_ {\frac{Z}{\sqrt{n}}} ( t ) )^n $ 

Since $Z_i \sim N(0,1)$, then $M_Z (t)= e^ \frac {t^2}{2} $

We can get $M_ {\frac{Z}{\sqrt{n}}} ( t )= e^ \frac {( \frac{t}{\sqrt{n}})^2}{2} = e^ \frac{t^2}{2n}$

$ M_{\frac{\sum_{i=1}^{n} (Z_i+ \frac{1}{n} ) }{\sqrt{n}} } (t)= E[e^  { \frac{1}{\sqrt{n}} \times t} ] \times (M_ {\frac{Z}{\sqrt{n}}} ( t ) )^n = e^ \frac{t}{\sqrt{n}} \times (e^ \frac{t^2}{2n})^n $
\par

$ = e^ \frac{t}{\sqrt{n}} \times e^ \frac{t^2}{2}  $

when n goes to infinity, $ e^ \frac{t}{\sqrt{n}} $ goes to 1. \par
So we have \par
$ \lim_{n \to \infty} M_{\frac{\sum_{i=1}^{n} (Z_i+ \frac{1}{n} ) }{\sqrt{n}} } (t) =  e^ \frac{t^2}{2} $ \par
which is the MGF of the normal distribution with mean 0 and variance 1 \par
we can conclude that $ \frac{\sum_{i=1}^{n} (Z_i+ \frac{1}{n} ) }{\sqrt{n}} \to X  \sim N(0,1)$ 
